Add eval fun

LeanScratch/Semantics/STLC/Red.lean
@@ -7,53 +7,68 @@ namespace STLC
 inductive Red : Stx → Stx → Prop
   | appl : Red a a' → Red (.app a b) (.app a' b)
   | appr : Red b b' → Red (.app a b) (.app a b')
+  | congr : Red a a' → Red (.abs ty a) (.abs ty a')
   | beta : Red (.app (.abs _ body) v) (body.β v)
 
-/- theorem refSet_maintain (h : Red a b) (hempty : a.refSet 0 = {}) : b.refSet 0 = {} := by -/
-/-   induction h -/
-/-   <;> simp_all [Stx.refSet, Nat.succ_eq_add_one, Stx.β, Stx.replace] -/
-/-   <;> obtain ⟨ha, hb⟩ := Finset.union_eq_empty.mp hempty -/
-/-   case appl h a_ih => -/
-/-     exact Finset.union_eq_empty.mpr ⟨a_ih ha, hb⟩ -/
-/-   case appr h a_ih => -/
-/-     exact Finset.union_eq_empty.mpr ⟨ha, a_ih hb⟩ -/
-/-   case beta x body v=> -/
-/-     induction body -/
-/-     <;> simp [Stx.refSet, Stx.replace, Stx.replace.bvar] -/
-/-     · split <;> (try split) -/
-/-       · exact hb -/
-/-       · simp_all only [Stx.refSet, Nat.lt_one_iff, ite_false, Finset.union_empty, -/
-/-           Finset.singleton_ne_empty] -/
-/-       next h => -/
-/-         simp only [not_lt, nonpos_iff_eq_zero] at h -/
-/-         contradiction -/
-/-     case app fn arg fn_ih arg_ih  => -/
-/-       sorry -/
-/-     case abs body' body_ih => -/
-/-       sorry -/
+@[simp]
+theorem Red_abs : Red (.abs ty body) a ↔ ∃ body', (Red body body') ∧ a = .abs ty body' := by
+  constructor
+  <;> intro h
+  · cases h; next body' h =>
+    use body'
+  · rcases h with ⟨body', h, rfl⟩
+    exact .congr h
+
+open Stx in
+theorem Red.VarFwd (r : Red a b) (next : RefSet b idx ) : RefSet a idx :=
+  match r with
+  | .appl h => by
+    simp only [RefSet_app] at next ⊢
+    match next with
+    | .inl h' => exact .inl $ Red.VarFwd h h'
+    | .inr h' => exact .inr h'
+  | .congr h => by
+    rw [RefSet_abs] at next ⊢
+    exact Red.VarFwd h next
+  | .appr h => by
+    simp only [RefSet_app] at next ⊢
+    match next with
+    | .inl h' => exact .inl h'
+    | .inr h' => exact .inr $ Red.VarFwd h h'
+  | .beta => STLC.Stx.VarFwd next
 
 abbrev RedStar := Relation.ReflTransGen Red
+abbrev RedPlus := Relation.TransGen Red
 
-def Ex.fstFn (a b : Ty) : Stx := .abs a (.abs b (.bvar 1))
-def Ex.sndFn (a b : Ty) : Stx := .abs a (.abs b (.bvar 0))
-def Ex.id (a : Ty) : Stx := .abs a (.bvar 0)
+mutual
+theorem Terminal_not_Red (terminal : Stx.Terminal a) : ¬Red a b := fun h =>
+  match h with
+  | .appl h => by
+    rw [Stx.Terminal_app] at terminal
+    rcases terminal with ⟨a, _⟩
+    exact NonEval_not_Red a h
+  | .appr h => by
+    rw [Stx.Terminal_app] at terminal
+    rcases terminal with ⟨_, a⟩
+    exact Terminal_not_Red a h
+  | .congr h => by
+    rw [Stx.Terminal_abs] at terminal
+    exact Terminal_not_Red terminal h
+  | .beta => by rcases terminal with (_|_|_|_)
+theorem NonEval_not_Red (terminal : Stx.NonEval a) : ¬Red a b := fun h =>
+  match h with
+  | .appl h => by
+    rw [Stx.NonEval_app] at terminal
+    rcases terminal with ⟨a, _⟩
+    exact NonEval_not_Red a h
+  | .appr h => by
+    rw [Stx.NonEval_app] at terminal
+    rcases terminal with ⟨_, a⟩
+    exact Terminal_not_Red a h
+  | .congr h => by
+    cases terminal
+  | .beta => by rcases terminal with (_|_|_)
+end
 
-def d0 := Ty.direct 0
-
-example : Red (.app (Ex.id d0) (.bvar n)) (.bvar n) := .beta
-example : Red (.app (Ex.id d0) z) z := by
-  have x : z = Stx.β (.bvar 0) z := by simp [Stx.β, Stx.replace, Stx.replace.bvar]
-  nth_rw 2 [x]
-  exact .beta
-example : Red (.app (Ex.sndFn d0 d0) x) (Ex.id d0) := .beta
-
-example : RedStar (.app (.app (Ex.fstFn d0 d0 ) a) b) a := by
-  have : RedStar (.app (.app (Ex.fstFn d0 d0 ) a) b) _ := .tail (.tail .refl (.appl .beta)) .beta
-  simp [Stx.replace, Stx.replace.bvar] at this
-  sorry
-/-   calc -/
-/-     RedStar _ (((Stx.abs d0 (Stx.bvar 1)).β (Stx.bvar 0)).app (Stx.bvar 1)) := .tail .refl (.appl .beta) -/
-/-     RedStar _ _ := sorry -/
-/- example : RedStar (.abs ) -/
-
+end STLC
 
