LeanScratch/Semantics/STLC/Step.lean
@@ -1,0 +1,94 @@
+import LeanScratch.Semantics.STLC.Stx
+import LeanScratch.Semantics.STLC.Red
+import Mathlib.Data.Rel
+import LeanScratch.Relation
+
+namespace STLC
+
+def step : Stx → Option Stx
+  | .bvar _ => .none
+  | .abs ty body => (step body).map (.abs ty ·)
+  | .app (.abs _ body) repl => .some $ body.β repl
+  | .app a b => match step a, step b with
+    | .none, .none => .none
+    | .some a, .none
+    | .none, .some b
+    | .some a, .some b => .some $ .app a b
+
+lemma RedPlus_congr (h : RedPlus body w) : RedPlus (.abs ty body) (.abs ty w) := by
+  induction h
+  case single h     => exact .single $ .congr h
+  case tail body ih => exact .tail ih $ .congr body
+
+lemma RedPlus_appl (h : RedPlus a w) : RedPlus (.app a b) (.app w b) := by
+  induction h
+  case single h     => exact .single $ .appl h
+  case tail body ih => exact .tail ih $ .appl body
+
+lemma RedPlus_appr (h : RedPlus a w) : RedPlus (.app b a) (.app b w) := by
+  induction h
+  case single h     => exact .single $ .appr h
+  case tail body ih => exact .tail ih $ .appr body
+
+theorem step_some_RedPlus (h : step main = .some a₁) : RedPlus main a₁ := 
+  match main with
+  | .bvar id => by simp only [step] at h
+  | .abs ty body => by
+    simp only [step, Option.map_eq_some'] at h
+    rcases h with ⟨w, h, rfl⟩
+    exact RedPlus_congr $ step_some_RedPlus h
+  | .app a b => by
+    by_cases isAbs : ∃ ty body, a = .abs ty body
+    · rcases isAbs with ⟨ty,body, rfl⟩
+      simp only [step, Option.some.injEq] at h
+      rw [←h]
+      exact .single .beta
+    · simp only [not_exists] at isAbs
+      unfold step at h
+      split at h
+      <;> try contradiction
+      next heq => simp_all only [Stx.app.injEq, false_and]
+      next heq =>
+        split at h
+        <;> simp only [Option.some.injEq] at h
+        <;> rw [←h, heq]
+        next a b _ _ _ a' ha hb =>
+          exact RedPlus_appl $ step_some_RedPlus ha
+        next ha hb =>
+          exact RedPlus_appr $ step_some_RedPlus hb
+        next a b _ _ _ a' b' ha hb =>
+          calc
+            RedPlus _ (.app _ _) := RedPlus_appr $ step_some_RedPlus hb
+            RedPlus _ (.app _ _) := RedPlus_appl $ step_some_RedPlus ha
+termination_by SizeOf.sizeOf main
+decreasing_by
+  all_goals simp_wf
+  <;> simp_all only [Stx.app.injEq, Option.some.injEq]
+  <;> linarith
+
+theorem step_none_terminal (h : step main = .none) : Stx.Terminal main :=
+  match main with
+  | .bvar id => .nonEval .bvar
+  | .abs ty body => by
+    simp only [step, Option.map_eq_none', Stx.Terminal_abs] at h ⊢
+    exact step_none_terminal h
+  | .app a b => by
+    by_cases isAbs : ∃ ty body, a = .abs ty body
+    · rcases isAbs with ⟨ty,body, rfl⟩
+      simp only [step] at h
+    · simp only [not_exists] at isAbs
+      unfold step at h
+      split at h
+      <;> try contradiction
+      split at h
+      <;> try contradiction
+      next heq _ _ ha hb =>
+      simp only [Stx.app.injEq] at heq
+      rcases heq with ⟨haa, hbb⟩
+      simp_all only [false_implies, implies_true, Stx.Terminal_app]
+      have ha := step_none_terminal ha
+      have hb := step_none_terminal hb
+      cases ha
+      · exfalso
+        exact isAbs _ _ rfl
+      next ha => exact ⟨ha, hb⟩
